src/theory/bir/bir_typing_expScript.sml
@@ -1,7 +1,7 @@
 open HolKernel Parse boolLib bossLib;
 open wordsTheory bitstringTheory;
 open optionTheory;
-open bir_auxiliaryTheory bir_immTheory bir_valuesTheory;
+open bir_auxiliaryTheory bir_immTheory bir_valuesTheory bir_env_oldTheory;
 open bir_exp_immTheory bir_exp_memTheory bir_envTheory;
 open bir_expTheory finite_mapTheory
 open pred_setTheory;
@@ -20,54 +20,50 @@ val bir_type_ss = rewrites (type_rws ``:bir_type_t``);
 
 
 val type_of_bir_exp_def = Define `
-  (type_of_bir_exp ext_map (BExp_Const i) = SOME (BType_Imm (type_of_bir_imm i))) /\
+  (type_of_bir_exp (BExp_Const i) = SOME (BType_Imm (type_of_bir_imm i))) /\
 
-  (type_of_bir_exp ext_map (BExp_MemConst aty vty mmap) = SOME (BType_Mem aty vty)) /\
+  (type_of_bir_exp (BExp_MemConst aty vty mmap) = SOME (BType_Mem aty vty)) /\
 
-  (type_of_bir_exp ext_map (BExp_Den v) = SOME (bir_var_type v)) /\
+  (type_of_bir_exp (BExp_Den v) = SOME (bir_var_type v)) /\
 
-  (type_of_bir_exp ext_map (BExp_Cast ct e rty) = (case (type_of_bir_exp ext_map e) of
+  (type_of_bir_exp (BExp_Cast ct e rty) = (case (type_of_bir_exp e) of
       NONE => NONE
     | SOME ty => (if (bir_type_is_Imm ty) then SOME (BType_Imm rty) else NONE))) /\
 
-  (type_of_bir_exp ext_map (BExp_UnaryExp et e) = (case (type_of_bir_exp ext_map e) of
+  (type_of_bir_exp (BExp_UnaryExp et e) = (case (type_of_bir_exp e) of
       NONE => NONE
     | SOME ty => (if (bir_type_is_Imm ty) then
         SOME ty else NONE))) /\
 
-  (type_of_bir_exp ext_map (BExp_BinExp et e1 e2) = (case (type_of_bir_exp ext_map e1,
-       type_of_bir_exp ext_map e2) of
+  (type_of_bir_exp (BExp_BinExp et e1 e2) = (case (type_of_bir_exp e1,
+       type_of_bir_exp e2) of
        (SOME ty1, SOME ty2) => (if ((bir_type_is_Imm ty1) /\ (ty2 = ty1)) then SOME ty1 else NONE)
        | _, _ => NONE)) /\
 
-  (type_of_bir_exp ext_map (BExp_BinPred pt e1 e2) = (case (type_of_bir_exp ext_map e1,
-       type_of_bir_exp ext_map e2) of
+  (type_of_bir_exp (BExp_BinPred pt e1 e2) = (case (type_of_bir_exp e1,
+       type_of_bir_exp e2) of
        (SOME ty1, SOME ty2) => (if ((bir_type_is_Imm ty1) /\ (ty2 = ty1)) then SOME BType_Bool else NONE)
        | _, _ => NONE)) /\
 
-  (type_of_bir_exp ext_map (BExp_MemEq e1 e2) = (case (type_of_bir_exp ext_map e1,
-       type_of_bir_exp ext_map e2) of
+  (type_of_bir_exp (BExp_MemEq e1 e2) = (case (type_of_bir_exp e1,
+       type_of_bir_exp e2) of
        (SOME (BType_Mem aty1 vty1), SOME (BType_Mem aty2 vty2)) => (if ((aty2 = aty1) /\ (vty2 = vty1)) then SOME BType_Bool else NONE)
        | _, _ => NONE)) /\
 
-
-  (type_of_bir_exp ext_map (BExp_IfThenElse ec e1 e2) = (case (type_of_bir_exp ext_map ec, type_of_bir_exp ext_map e1,
-       type_of_bir_exp ext_map e2) of
+  (type_of_bir_exp (BExp_IfThenElse ec e1 e2) = (case (type_of_bir_exp ec, type_of_bir_exp e1,
+       type_of_bir_exp e2) of
        (SOME ect, SOME ty1, SOME ty2) => (if ((ect = BType_Bool) /\ (ty2 = ty1)) then SOME ty1 else NONE)
        | _, _, _ => NONE)) /\
 
-  (type_of_bir_exp ext_map (BExp_ExtGet ext_name ty) =
-    case FLOOKUP (FST ext_map) ext_name of
-    | SOME v => if type_of_bir_val v = ty then SOME ty else NONE
-    | NONE => NONE) /\
+  (type_of_bir_exp (BExp_ExtGet ext_name ty) = SOME ty) /\
 
-  (type_of_bir_exp ext_map (BExp_Load me ae en rty) = (case (type_of_bir_exp ext_map me, type_of_bir_exp ext_map ae) of
+  (type_of_bir_exp (BExp_Load me ae en rty) = (case (type_of_bir_exp me, type_of_bir_exp ae) of
        (SOME (BType_Mem aty vty), SOME (BType_Imm aty')) => (if (
             (aty = aty') /\ (if en = BEnd_NoEndian then (vty = rty) else (bir_number_of_mem_splits vty rty aty <> NONE))
            ) then SOME (BType_Imm rty) else NONE)
        | _, _ => NONE)) /\
 
-  (type_of_bir_exp ext_map (BExp_Store me ae en v) = (case (type_of_bir_exp ext_map me, type_of_bir_exp ext_map ae, type_of_bir_exp ext_map v) of
+  (type_of_bir_exp (BExp_Store me ae en v) = (case (type_of_bir_exp me, type_of_bir_exp ae, type_of_bir_exp v) of
        (SOME (BType_Mem aty vty), SOME (BType_Imm aty'), SOME (BType_Imm rty)) => (if (
             (aty = aty') /\ (if en = BEnd_NoEndian then (vty = rty) else (bir_number_of_mem_splits vty rty aty <> NONE))
            ) then SOME (BType_Mem aty vty) else NONE)
@@ -76,7 +72,7 @@ val type_of_bir_exp_def = Define `
 
 
 val type_of_bir_exp_THM = store_thm ("type_of_bir_exp_THM",
- ``!ext_map ext_st env e ty. (type_of_bir_exp ext_map e = SOME ty) ==>
+ ``!(ext_map:'ext_state_t bir_ext_map_t) ext_st env e ty. (type_of_bir_exp e = SOME ty) ==>
               ((bir_eval_exp ext_map e env ext_st = NONE) \/
                (?v. (bir_eval_exp ext_map e env ext_st = SOME v) /\ (type_of_bir_val v = ty)))``,
 
@@ -123,7 +119,10 @@ Induct >> (
 ) >- (
   fs[bir_eval_extget_def] >>
   rpt strip_tac >>
-  Cases_on `FLOOKUP (FST ext_map) s` >> (
+  Cases_on `bir_lookup_get ext_map s` >> (
+    fs []
+  ) >>
+  Cases_on `x ext_st` >> (
     fs []
   )
 ) >- (
@@ -140,47 +139,46 @@ Induct >> (
 
 
 val type_of_bir_exp_EQ_SOME_REWRS = store_thm ("type_of_bir_exp_EQ_SOME_REWRS",``
-  (!ext_map i ty. (type_of_bir_exp ext_map (BExp_Const i) = SOME ty) <=> (ty = BType_Imm (type_of_bir_imm i))) /\
+  (!i ty. (type_of_bir_exp (BExp_Const i) = SOME ty) <=> (ty = BType_Imm (type_of_bir_imm i))) /\
 
-  (!ext_map aty vty mmap ty. (type_of_bir_exp ext_map (BExp_MemConst aty vty mmap) = SOME ty) <=> (ty = BType_Mem aty vty)) /\
+  (!aty vty mmap ty. (type_of_bir_exp (BExp_MemConst aty vty mmap) = SOME ty) <=> (ty = BType_Mem aty vty)) /\
 
-  (!ext_map v ty. (type_of_bir_exp ext_map (BExp_Den v) = SOME ty) <=> (ty = bir_var_type v)) /\
+  (!v ty. (type_of_bir_exp (BExp_Den v) = SOME ty) <=> (ty = bir_var_type v)) /\
 
-  (!ext_map ct e ty ty'. (type_of_bir_exp ext_map (BExp_Cast ct e ty') = SOME ty) <=> (
-     (ty = BType_Imm ty') /\ (?it. (type_of_bir_exp ext_map e = SOME (BType_Imm it))))) /\
+  (!ct e ty ty'. (type_of_bir_exp (BExp_Cast ct e ty') = SOME ty) <=> (
+     (ty = BType_Imm ty') /\ (?it. (type_of_bir_exp e = SOME (BType_Imm it))))) /\
 
-  (!ext_map et e ty. (type_of_bir_exp ext_map (BExp_UnaryExp et e) = SOME ty) <=> (
-     (bir_type_is_Imm ty) /\ (type_of_bir_exp ext_map e = SOME ty))) /\
+  (!et e ty. (type_of_bir_exp (BExp_UnaryExp et e) = SOME ty) <=> (
+     (bir_type_is_Imm ty) /\ (type_of_bir_exp e = SOME ty))) /\
 
-  (!ext_map et e1 e2 ty. (type_of_bir_exp ext_map (BExp_BinExp et e1 e2) = SOME ty) <=> (
-     (bir_type_is_Imm ty) /\ (type_of_bir_exp ext_map e1 = SOME ty) /\ (type_of_bir_exp ext_map e2 = SOME ty))) /\
+  (!et e1 e2 ty. (type_of_bir_exp (BExp_BinExp et e1 e2) = SOME ty) <=> (
+     (bir_type_is_Imm ty) /\ (type_of_bir_exp e1 = SOME ty) /\ (type_of_bir_exp e2 = SOME ty))) /\
 
-  (!ext_map pt e1 e2 ty. (type_of_bir_exp ext_map (BExp_BinPred pt e1 e2) = SOME ty) <=> (
-     (ty = BType_Bool) /\ (?it. (type_of_bir_exp ext_map e1 = SOME (BType_Imm it)) /\
-                              (type_of_bir_exp ext_map e2 = SOME (BType_Imm it))))) /\
+  (!pt e1 e2 ty. (type_of_bir_exp (BExp_BinPred pt e1 e2) = SOME ty) <=> (
+     (ty = BType_Bool) /\ (?it. (type_of_bir_exp e1 = SOME (BType_Imm it)) /\
+                              (type_of_bir_exp e2 = SOME (BType_Imm it))))) /\
 
-  (!ext_map me1 me2 ty. (type_of_bir_exp ext_map (BExp_MemEq me1 me2) = SOME ty) <=> (
-     ?at vt. (ty = BType_Bool) /\ (type_of_bir_exp ext_map me1 = SOME (BType_Mem at vt)) /\ (type_of_bir_exp ext_map me2 = type_of_bir_exp ext_map me1))) /\
+  (!me1 me2 ty. (type_of_bir_exp (BExp_MemEq me1 me2) = SOME ty) <=> (
+     ?at vt. (ty = BType_Bool) /\ (type_of_bir_exp me1 = SOME (BType_Mem at vt)) /\ (type_of_bir_exp me2 = type_of_bir_exp me1))) /\
 
-  (!ext_map ce e1 e2 ty. (type_of_bir_exp ext_map (BExp_IfThenElse ce e1 e2) = SOME ty) <=> (
-     (type_of_bir_exp ext_map ce = SOME BType_Bool) /\
-     (type_of_bir_exp ext_map e1 = SOME ty) /\
-     (type_of_bir_exp ext_map e2 = SOME ty))) /\
+  (!ce e1 e2 ty. (type_of_bir_exp (BExp_IfThenElse ce e1 e2) = SOME ty) <=> (
+     (type_of_bir_exp ce = SOME BType_Bool) /\
+     (type_of_bir_exp e1 = SOME ty) /\
+     (type_of_bir_exp e2 = SOME ty))) /\
 
-  (!ext_map ext_name ty ty'. (type_of_bir_exp ext_map (BExp_ExtGet ext_name ty) = SOME ty') <=> (
-     ty = ty' /\ (?v. FLOOKUP (FST ext_map) ext_name = SOME v /\ type_of_bir_val v = ty))) /\
+  (!ext_name ty ty'. (type_of_bir_exp (BExp_ExtGet ext_name ty) = SOME ty') <=> (ty = ty')) /\
 
-  (!ext_map rty ty ae en me. (type_of_bir_exp ext_map (BExp_Load me ae en rty) = SOME ty) <=> (
-     (ty = BType_Imm rty) /\ (?at vt. (type_of_bir_exp ext_map me = SOME (BType_Mem at vt)) /\
-                            (type_of_bir_exp ext_map ae = SOME (BType_Imm at)) /\
+  (!rty ty ae en me. (type_of_bir_exp (BExp_Load me ae en rty) = SOME ty) <=> (
+     (ty = BType_Imm rty) /\ (?at vt. (type_of_bir_exp me = SOME (BType_Mem at vt)) /\
+                            (type_of_bir_exp ae = SOME (BType_Imm at)) /\
                             (if en = BEnd_NoEndian then (vt = rty) else
                                   (bir_number_of_mem_splits vt rty at <> NONE))))) /\
 
-  (!ext_map ty ae en me v. (type_of_bir_exp ext_map (BExp_Store me ae en v) = SOME ty) <=> (
+  (!ty ae en me v. (type_of_bir_exp (BExp_Store me ae en v) = SOME ty) <=> (
      ?at vt rty. (ty = BType_Mem at vt) /\
-             (type_of_bir_exp ext_map me = SOME (BType_Mem at vt)) /\
-             (type_of_bir_exp ext_map ae = SOME (BType_Imm at)) /\
-             (type_of_bir_exp ext_map v = SOME (BType_Imm rty)) /\
+             (type_of_bir_exp me = SOME (BType_Mem at vt)) /\
+             (type_of_bir_exp ae = SOME (BType_Imm at)) /\
+             (type_of_bir_exp v = SOME (BType_Imm rty)) /\
              (if en = BEnd_NoEndian then (vt = rty) else
                                   (bir_number_of_mem_splits vt rty at <> NONE))))
 ``,
@@ -212,17 +210,15 @@ REPEAT CONJ_TAC >> (
   REPEAT GEN_TAC >> REPEAT CASE_TAC >> METIS_TAC[]
 ) >- (
   REPEAT GEN_TAC >> REPEAT CASE_TAC >> METIS_TAC[]
-) >- (
-  REPEAT GEN_TAC >> REPEAT CASE_TAC >> METIS_TAC[]
 ));
 
 
 val bir_eval_exp_IS_SOME_IMPLIES_TYPE =
   store_thm("bir_eval_exp_IS_SOME_IMPLIES_TYPE",
-  ``!ext_map env ext_st e va ty.
+  ``!(ext_map:'ext_state_t bir_ext_map_t) env ext_st e va ty.
     (bir_eval_exp ext_map e env ext_st = SOME va) ==>
     (type_of_bir_val va = ty) ==>
-    (type_of_bir_exp ext_map e = SOME ty)``,
+    (type_of_bir_exp e = SOME ty)``,
 
 Induct_on `e` >> (
   REPEAT STRIP_TAC >>
@@ -308,7 +304,10 @@ Induct_on `e` >> (
 
   (* ExtGet *)
   fs [bir_eval_extget_def] >>
-  Cases_on `FLOOKUP (FST ext_map) s` >> (
+  Cases_on `bir_lookup_get ext_map s` >> (
+    fs[]
+  ) >>
+  Cases_on `x ext_st` >> (
     gvs[]
   ),
 
@@ -372,50 +371,48 @@ Induct_on `e` >> (
 
 
 val type_of_bir_exp_EQ_NONE_REWRS = store_thm ("type_of_bir_exp_EQ_NONE_REWRS",``
-  (!ext_map i. ~(type_of_bir_exp ext_map (BExp_Const i) = NONE)) /\
+  (!i. ~(type_of_bir_exp (BExp_Const i) = NONE)) /\
 
-  (!ext_map aty vty mmap. ~(type_of_bir_exp ext_map (BExp_MemConst aty vty mmap) = NONE)) /\
+  (!aty vty mmap. ~(type_of_bir_exp (BExp_MemConst aty vty mmap) = NONE)) /\
 
-  (!ext_map v. ~(type_of_bir_exp ext_map (BExp_Den v) = NONE)) /\
+  (!v. ~(type_of_bir_exp (BExp_Den v) = NONE)) /\
 
-  (!ext_map ct e ty ty'. (type_of_bir_exp ext_map (BExp_Cast ct e ty') = NONE) <=> (
-     (!ity. (type_of_bir_exp ext_map e <> SOME (BType_Imm ity))))) /\
+  (!ct e ty. (type_of_bir_exp (BExp_Cast ct e ty) = NONE) <=> (
+     (!ity. (type_of_bir_exp e <> SOME (BType_Imm ity))))) /\
 
-  (!ext_map et e. (type_of_bir_exp ext_map (BExp_UnaryExp et e) = NONE) <=> (
-     (!ity. type_of_bir_exp ext_map e <> SOME (BType_Imm ity)))) /\
+  (!et e. (type_of_bir_exp (BExp_UnaryExp et e) = NONE) <=> (
+     (!ity. type_of_bir_exp e <> SOME (BType_Imm ity)))) /\
 
-  (!ext_map et e1 e2. (type_of_bir_exp ext_map (BExp_BinExp et e1 e2) = NONE) <=> !ity.
-     (type_of_bir_exp ext_map e1 <> SOME (BType_Imm ity)) \/
-     (type_of_bir_exp ext_map e2 <> SOME (BType_Imm ity))) /\
+  (!et e1 e2. (type_of_bir_exp (BExp_BinExp et e1 e2) = NONE) <=> !ity.
+     (type_of_bir_exp e1 <> SOME (BType_Imm ity)) \/
+     (type_of_bir_exp e2 <> SOME (BType_Imm ity))) /\
 
-  (!ext_map pt e1 e2. (type_of_bir_exp ext_map (BExp_BinPred pt e1 e2) = NONE) <=> !ity.
-     (type_of_bir_exp ext_map e1 <> SOME (BType_Imm ity)) \/
-     (type_of_bir_exp ext_map e2 <> SOME (BType_Imm ity))) /\
+  (!pt e1 e2. (type_of_bir_exp (BExp_BinPred pt e1 e2) = NONE) <=> !ity.
+     (type_of_bir_exp e1 <> SOME (BType_Imm ity)) \/
+     (type_of_bir_exp e2 <> SOME (BType_Imm ity))) /\
 
-  (!ext_map me1 me2. (type_of_bir_exp ext_map (BExp_MemEq me1 me2) = NONE) <=> !at vt.
-     (type_of_bir_exp ext_map me1 <> SOME (BType_Mem at vt)) \/
-     (type_of_bir_exp ext_map me2 <> SOME (BType_Mem at vt))) /\
+  (!me1 me2. (type_of_bir_exp (BExp_MemEq me1 me2) = NONE) <=> !at vt.
+     (type_of_bir_exp me1 <> SOME (BType_Mem at vt)) \/
+     (type_of_bir_exp me2 <> SOME (BType_Mem at vt))) /\
 
-  (!ext_map ce e1 e2 ty. (type_of_bir_exp ext_map (BExp_IfThenElse ce e1 e2) = NONE) <=> (
-     (type_of_bir_exp ext_map ce <> SOME BType_Bool) \/
-     (type_of_bir_exp ext_map e1 = NONE) \/
-     (type_of_bir_exp ext_map e2 <> type_of_bir_exp ext_map e1))) /\
+  (!ce e1 e2. (type_of_bir_exp (BExp_IfThenElse ce e1 e2) = NONE) <=> (
+     (type_of_bir_exp ce <> SOME BType_Bool) \/
+     (type_of_bir_exp e1 = NONE) \/
+     (type_of_bir_exp e2 <> type_of_bir_exp e1))) /\
 
-  (!ext_map en ty. (type_of_bir_exp ext_map (BExp_ExtGet en ty) = NONE) <=> (
-     (FLOOKUP (FST ext_map) en = NONE) \/
-     (?v. FLOOKUP (FST ext_map) en = SOME v /\ type_of_bir_val v <> ty))) /\
+  (!en ty. ~(type_of_bir_exp (BExp_ExtGet en ty) = NONE)) /\
 
-  (!ext_map rty ty ae en me. (type_of_bir_exp ext_map (BExp_Load me ae en rty) = NONE) <=> (
-     (!at vt. (type_of_bir_exp ext_map me = SOME (BType_Mem at vt)) /\
-              (type_of_bir_exp ext_map ae = SOME (BType_Imm at)) ==>
+  (!rty ae en me. (type_of_bir_exp (BExp_Load me ae en rty) = NONE) <=> (
+     (!at vt. (type_of_bir_exp me = SOME (BType_Mem at vt)) /\
+              (type_of_bir_exp ae = SOME (BType_Imm at)) ==>
               (if en = BEnd_NoEndian then (vt <> rty) else
                    (bir_number_of_mem_splits vt rty at = NONE))))) /\
 
-  (!ext_map ty ae en me v. (type_of_bir_exp ext_map (BExp_Store me ae en v) = NONE) <=> (
+  (!ae en me v. (type_of_bir_exp (BExp_Store me ae en v) = NONE) <=> (
      !at vt rty.
-             (type_of_bir_exp ext_map me = SOME (BType_Mem at vt)) /\
-             (type_of_bir_exp ext_map ae = SOME (BType_Imm at)) /\
-             (type_of_bir_exp ext_map v = SOME (BType_Imm rty)) ==>
+             (type_of_bir_exp me = SOME (BType_Mem at vt)) /\
+             (type_of_bir_exp ae = SOME (BType_Imm at)) /\
+             (type_of_bir_exp v = SOME (BType_Imm rty)) ==>
              (if en = BEnd_NoEndian then (vt <> rty) else
                                   (bir_number_of_mem_splits vt rty at = NONE))))
 ``,
@@ -445,9 +442,7 @@ REPEAT CONJ_TAC >> (
   REPEAT GEN_TAC >> REPEAT CASE_TAC >> (
     FULL_SIMP_TAC (std_ss) []
   )
-) >- (
-  REPEAT GEN_TAC >> REPEAT CASE_TAC >> METIS_TAC[]
-) >- (
+)  >- (
   REPEAT GEN_TAC >> REPEAT CASE_TAC >> METIS_TAC[]
 ) >- (
   REPEAT GEN_TAC >> REPEAT CASE_TAC >> METIS_TAC[]
@@ -455,14 +450,14 @@ REPEAT CONJ_TAC >> (
 
 
 val type_of_bir_exp_NOT_SOME_Imm = prove(
-  ``!ext_map ex env. 
-    (!ity. type_of_bir_exp ext_map ex <> SOME (BType_Imm ity)) ==>
-    (?aty vty. (type_of_bir_exp ext_map ex = SOME (BType_Mem aty vty)) \/
-     (type_of_bir_exp ext_map ex = NONE)
+  ``!ex. 
+    (!ity. type_of_bir_exp ex <> SOME (BType_Imm ity)) ==>
+    (?aty vty. (type_of_bir_exp ex = SOME (BType_Mem aty vty)) \/
+     (type_of_bir_exp ex = NONE)
     )``,
 
 REPEAT STRIP_TAC >>
-Cases_on `type_of_bir_exp ext_map ex` >> (
+Cases_on `type_of_bir_exp ex` >> (
   FULL_SIMP_TAC (std_ss) []
 ) >>
 Cases_on `x` >> (
@@ -471,26 +466,26 @@ Cases_on `x` >> (
 );
 
 val type_of_2bir_exp_NOT_SOME_Imm = prove(
-  ``!ext_map ex ex'. 
+  ``!ex ex'. 
     (!ity.
-     type_of_bir_exp ext_map ex <> SOME (BType_Imm ity) \/
-     type_of_bir_exp ext_map ex' <> SOME (BType_Imm ity)) ==>
-    ((?aty vty. type_of_bir_exp ext_map ex = SOME (BType_Mem aty vty)) \/
-     (type_of_bir_exp ext_map ex = NONE) \/
-     (?aty vty. type_of_bir_exp ext_map ex' = SOME (BType_Mem aty vty)) \/
-     (type_of_bir_exp ext_map ex' = NONE) \/
+     type_of_bir_exp ex <> SOME (BType_Imm ity) \/
+     type_of_bir_exp ex' <> SOME (BType_Imm ity)) ==>
+    ((?aty vty. type_of_bir_exp ex = SOME (BType_Mem aty vty)) \/
+     (type_of_bir_exp ex = NONE) \/
+     (?aty vty. type_of_bir_exp ex' = SOME (BType_Mem aty vty)) \/
+     (type_of_bir_exp ex' = NONE) \/
      (?ity' ity''.
-      (type_of_bir_exp ext_map ex = SOME (BType_Imm ity')) /\
-      (type_of_bir_exp ext_map ex' = SOME (BType_Imm ity'')) /\
+      (type_of_bir_exp ex = SOME (BType_Imm ity')) /\
+      (type_of_bir_exp ex' = SOME (BType_Imm ity'')) /\
       (ity' <> ity'')
      )
     )``,
 
 REPEAT STRIP_TAC >>
-Cases_on `type_of_bir_exp ext_map ex` >> (
+Cases_on `type_of_bir_exp ex` >> (
   FULL_SIMP_TAC std_ss []
 ) >>
-Cases_on `type_of_bir_exp ext_map ex'` >> (
+Cases_on `type_of_bir_exp ex'` >> (
   FULL_SIMP_TAC std_ss []
 ) >>
 Cases_on `x` >> Cases_on `x'` >> (
@@ -499,8 +494,8 @@ Cases_on `x` >> Cases_on `x'` >> (
 );
 
 val bir_type_of_bir_exp_NONE = store_thm("bir_type_of_bir_exp_NONE",
-  ``!ext_map ex env ext_st.
-    (type_of_bir_exp ext_map ex = NONE) ==>
+  ``!(ext_map:'ext_state_t bir_ext_map_t) ex env ext_st.
+    (type_of_bir_exp ex = NONE) ==>
     (bir_eval_exp ext_map ex env ext_st = NONE)``,
 
 REPEAT STRIP_TAC >>
@@ -514,7 +509,7 @@ Induct_on `ex` >> (
   ) >>
   (* The memory remains... *)
   IMP_RES_TAC type_of_bir_exp_THM >>
-  QSPECL_X_ASSUM ``!ext_st env. _`` [`ext_st`, `env`] >>
+  QSPECL_X_ASSUM ``!ext_st ext_map env. _`` [`ext_st`, `ext_map`, `env`] >>
   FULL_SIMP_TAC std_ss [bir_eval_cast_REWRS] >>
   Cases_on `v` >> (
     FULL_SIMP_TAC (std_ss++bir_type_ss) [bir_eval_cast_REWRS, type_of_bir_val_def]
@@ -525,7 +520,7 @@ Induct_on `ex` >> (
     FULL_SIMP_TAC std_ss [bir_eval_unary_exp_REWRS]
   ) >>
   IMP_RES_TAC type_of_bir_exp_THM >>
-  QSPECL_X_ASSUM ``!ext_st env. _`` [`ext_st`, `env`] >>
+  QSPECL_X_ASSUM ``!ext_st ext_map env. _`` [`ext_st`, `ext_map`, `env`] >>
   FULL_SIMP_TAC std_ss [bir_eval_unary_exp_REWRS] >>
   Cases_on `v` >> (
     FULL_SIMP_TAC (std_ss++bir_type_ss) [bir_eval_unary_exp_REWRS, type_of_bir_val_def]
@@ -538,8 +533,8 @@ Induct_on `ex` >> (
     IMP_RES_TAC type_of_bir_exp_THM
   ) >> (
     (* 3 cases, two of which are proved by the below: *)
-    QSPECL_X_ASSUM ``!ext_st env. _`` [`ext_st`, `env`] >>
-    TRY (QSPECL_X_ASSUM ``!ext_st env. _`` [`ext_st`, `env`]) >>
+    QSPECL_X_ASSUM ``!ext_st ext_map env. _`` [`ext_st`, `ext_map`, `env`] >>
+    TRY (QSPECL_X_ASSUM ``!ext_st ext_map env. _`` [`ext_st`, `ext_map`, `env`]) >>
     FULL_SIMP_TAC std_ss [bir_eval_bin_exp_REWRS] >>
     Cases_on `v` >> (
       FULL_SIMP_TAC (std_ss++bir_type_ss) [bir_eval_bin_exp_REWRS, type_of_bir_val_def]
@@ -556,8 +551,8 @@ Induct_on `ex` >> (
   ) >> (
     IMP_RES_TAC type_of_bir_exp_THM
   ) >> (
-    QSPECL_X_ASSUM ``!ext_st env. _`` [`ext_st`, `env`] >>
-    TRY (QSPECL_X_ASSUM ``!ext_st env. _`` [`ext_st`, `env`]) >>
+    QSPECL_X_ASSUM ``!ext_st ext_map env. _`` [`ext_st`, `ext_map`, `env`] >>
+    TRY (QSPECL_X_ASSUM ``!ext_st ext_map env. _`` [`ext_st`, `ext_map`, `env`]) >>
     FULL_SIMP_TAC std_ss [bir_eval_bin_pred_REWRS] >>
     Cases_on `v` >> (
       FULL_SIMP_TAC (std_ss++bir_type_ss) [bir_eval_bin_pred_REWRS, type_of_bir_val_def]
@@ -568,13 +563,13 @@ Induct_on `ex` >> (
   ),
 
   (* MemEq *)
-  Cases_on `type_of_bir_exp ext_map ex` >> Cases_on `type_of_bir_exp ext_map ex'` >> (
+  Cases_on `type_of_bir_exp ex` >> Cases_on `type_of_bir_exp ex'` >> (
     FULL_SIMP_TAC std_ss [bir_eval_memeq_REWRS]
   ) >>
   IMP_RES_TAC type_of_bir_exp_THM >>
   Cases_on `x` >> Cases_on `x'` >> (
     FULL_SIMP_TAC (std_ss++bir_type_ss) [] >>
-    REPEAT (QSPECL_X_ASSUM ``!ext_st env. _`` [`ext_st`, `env`]) >>
+    REPEAT (QSPECL_X_ASSUM ``!ext_st ext_map env. _`` [`ext_st`, `ext_map`, `env`]) >>
     FULL_SIMP_TAC std_ss [bir_eval_memeq_REWRS]
   ) >> (
     Cases_on `v` >> (
@@ -587,39 +582,33 @@ Induct_on `ex` >> (
 
   (* IfThenElse condition *)
   FULL_SIMP_TAC std_ss [BType_Bool_def] >>
-  Cases_on `type_of_bir_exp ext_map ex` >> (
+  Cases_on `type_of_bir_exp ex` >> (
     FULL_SIMP_TAC (std_ss++bir_type_ss) [bir_eval_ifthenelse_REWRS]
   ) >>
   IMP_RES_TAC type_of_bir_exp_THM >>
-  QSPECL_X_ASSUM ``!ext_st env. _`` [`ext_st`, `env`] >>
+  QSPECL_X_ASSUM ``!ext_st ext_map env. _`` [`ext_st`, `ext_map`, `env`] >>
   FULL_SIMP_TAC std_ss [bir_eval_ifthenelse_REWRS, bir_eval_ifthenelse_REWRS_NONE],
 
   (* IfThenElse second argument NONE *)
   FULL_SIMP_TAC std_ss [bir_eval_ifthenelse_REWRS],
 
   (* IfThenElse type mismatch *)
-  Cases_on `type_of_bir_exp ext_map ex'` >> (
+  Cases_on `type_of_bir_exp ex'` >> (
     FULL_SIMP_TAC std_ss [bir_eval_ifthenelse_REWRS]
   ) >>
-  Cases_on `type_of_bir_exp ext_map ex''` >> (
+  Cases_on `type_of_bir_exp ex''` >> (
     FULL_SIMP_TAC std_ss [bir_eval_ifthenelse_REWRS]
   ) >>
   IMP_RES_TAC type_of_bir_exp_THM >>
-  REPEAT (QSPECL_X_ASSUM ``!ext_st env. _`` [`ext_st`, `env`]) >>
+  REPEAT (QSPECL_X_ASSUM ``!ext_st ext_map env. _`` [`ext_st`, `ext_map`, `env`]) >>
   FULL_SIMP_TAC std_ss [bir_eval_ifthenelse_REWRS, bir_eval_ifthenelse_REWRS_NONE],
 
-  (* ExtGet - NONE *)
-  fs[bir_eval_extget_def],
-
-  (* ExtGet - SOME *)
-  fs[bir_eval_extget_def],
-
   (* Load *)
-  Cases_on `type_of_bir_exp ext_map ex` >> Cases_on `type_of_bir_exp ext_map ex'` >> (
+  Cases_on `type_of_bir_exp ex` >> Cases_on `type_of_bir_exp ex'` >> (
     FULL_SIMP_TAC std_ss [bir_eval_load_NONE_REWRS]
   ) >>
   IMP_RES_TAC type_of_bir_exp_THM >>
-  NTAC 2 (QSPECL_X_ASSUM ``!ext_st env. _`` [`ext_st`, `env`]) >>
+  NTAC 2 (QSPECL_X_ASSUM ``!ext_st ext_map env. _`` [`ext_st`, `ext_map`, `env`]) >>
   FULL_SIMP_TAC std_ss [bir_eval_load_NONE_REWRS] >>
   Cases_on `v` >> Cases_on `v'` >> (
     FULL_SIMP_TAC std_ss [bir_eval_load_NONE_REWRS]
@@ -638,12 +627,12 @@ Induct_on `ex` >> (
   ),
 
   (* Store *)
-  Cases_on `type_of_bir_exp ext_map ex` >> Cases_on `type_of_bir_exp ext_map ex'` >>
-    Cases_on `type_of_bir_exp ext_map ex''` >> (
+  Cases_on `type_of_bir_exp ex` >> Cases_on `type_of_bir_exp ex'` >>
+    Cases_on `type_of_bir_exp ex''` >> (
     FULL_SIMP_TAC std_ss [bir_eval_store_NONE_REWRS]
   ) >>
   IMP_RES_TAC type_of_bir_exp_THM >>
-  NTAC 3 (QSPECL_X_ASSUM ``!ext_st env. _`` [`ext_st`, `env`]) >>
+  NTAC 3 (QSPECL_X_ASSUM ``!ext_st ext_map env. _`` [`ext_st`, `ext_map`, `env`]) >>
   FULL_SIMP_TAC std_ss [bir_eval_store_NONE_REWRS] >>
   Cases_on `v` >> Cases_on `v'` >> Cases_on `v''` >> (
     FULL_SIMP_TAC std_ss [bir_eval_store_NONE_REWRS]
@@ -665,7 +654,7 @@ Induct_on `ex` >> (
 
 
 (* ------------------------------------------------------------------------- *)
-(*  Looking at  variables used somewhere in an expression                    *)
+(*  Looking at variables used somewhere in an expression                     *)
 (* ------------------------------------------------------------------------- *)
 
 val bir_vars_of_exp_def = Define `
@@ -684,7 +673,7 @@ val bir_vars_of_exp_def = Define `
 
 
 val bir_vars_of_exp_THM = store_thm ("bir_vars_of_exp_THM",
-``!env1 env2 e ext_map ext_st. (!v. v IN (bir_vars_of_exp e) ==>
+``!env1 env2 e (ext_map:'ext_state_t bir_ext_map_t) ext_st. (!v. v IN (bir_vars_of_exp e) ==>
                      (bir_env_read v env1 = bir_env_read v env2)) ==>
                 (bir_eval_exp ext_map e env1 ext_st = bir_eval_exp ext_map e env2 ext_st)``,
 
@@ -696,7 +685,7 @@ NTAC 2 GEN_TAC >> Induct >> REPEAT STRIP_TAC >> (
 
 
 val bir_vars_of_exp_THM_EQ_FOR_VARS = store_thm ("bir_vars_of_exp_THM_EQ_FOR_VARS",
-``!ext_map env1 env2 e ext_st. (bir_env_EQ_FOR_VARS (bir_vars_of_exp e) env1 env2) ==>
+``!(ext_map:'ext_state_t bir_ext_map_t) env1 env2 e ext_st. (bir_env_EQ_FOR_VARS (bir_vars_of_exp e) env1 env2) ==>
                 (bir_eval_exp ext_map e env1 ext_st = bir_eval_exp ext_map e env2 ext_st)``,
 METIS_TAC[bir_vars_of_exp_THM, bir_env_EQ_FOR_VARS_read_IMPL]);
 
@@ -711,17 +700,36 @@ Induct >> (
 ));
 
 
-val type_of_bir_exp_THM_with_envty = store_thm ("type_of_bir_exp_THM_with_envty",
-  ``!ext_map env ext_st envty e ty. (type_of_bir_exp ext_map e = SOME ty) ==>
-                     (bir_envty_includes_vs envty (bir_vars_of_exp e)) ==>
-                     (bir_env_satisfies_envty env envty) ==>
-                     (?v. ((bir_eval_exp ext_map e env ext_st) = SOME v) /\ (type_of_bir_val v = ty))``,
+val bir_exts_of_exp_def = Define `
+  (bir_exts_of_exp (BExp_Const _) = {}) /\
+  (bir_exts_of_exp (BExp_MemConst _ _ _) = {}) /\
+  (bir_exts_of_exp (BExp_Den v) = {}) /\
+  (bir_exts_of_exp (BExp_Cast _ e _) = bir_exts_of_exp e) /\
+  (bir_exts_of_exp (BExp_UnaryExp _ e) = bir_exts_of_exp e) /\
+  (bir_exts_of_exp (BExp_BinExp _ e1 e2) = (bir_exts_of_exp e1 UNION bir_exts_of_exp e2)) /\
+  (bir_exts_of_exp (BExp_BinPred _ e1 e2) = (bir_exts_of_exp e1 UNION bir_exts_of_exp e2)) /\
+  (bir_exts_of_exp (BExp_MemEq e1 e2) = (bir_exts_of_exp e1 UNION bir_exts_of_exp e2)) /\
+  (bir_exts_of_exp (BExp_IfThenElse ec e1 e2) = (bir_exts_of_exp ec UNION bir_exts_of_exp e1 UNION bir_exts_of_exp e2)) /\
+  (bir_exts_of_exp (BExp_ExtGet en ty) = {(en,ty)}) /\
+  (bir_exts_of_exp (BExp_Load me ae _ _) = (bir_exts_of_exp me UNION bir_exts_of_exp ae)) /\
+  (bir_exts_of_exp (BExp_Store me ae _ ve) = (bir_exts_of_exp me UNION bir_exts_of_exp ae UNION bir_exts_of_exp ve))`;
 
-NTAC 4 GEN_TAC >> Induct >> (
+
+val type_of_bir_exp_THM_with_envty = store_thm ("type_of_bir_exp_THM_with_envty",
+  ``!(ext_map:'ext_state_t bir_ext_map_t) env ext_st envty ext_envty e ty.
+    type_of_bir_exp e = SOME ty ==>
+    bir_envty_includes_vs envty (bir_vars_of_exp e) ==>
+    bir_env_satisfies_envty env envty ==>
+    bir_ext_envty_includes_exts ext_envty (bir_exts_of_exp e) ==>
+    bir_ext_env_satisfies_ext_envty (ext_map, ext_st) ext_envty ==>
+    ?v. bir_eval_exp ext_map e env ext_st = SOME v /\ type_of_bir_val v = ty``,
+
+NTAC 5 GEN_TAC >> Induct >> (
   SIMP_TAC (std_ss++bir_val_ss) [bir_eval_exp_def, BType_Bool_def,
-    type_of_bir_exp_EQ_SOME_REWRS, bir_vars_of_exp_def,
+    type_of_bir_exp_EQ_SOME_REWRS, bir_vars_of_exp_def, bir_exts_of_exp_def,
     bir_envty_includes_vs_UNION, bir_envty_includes_vs_INSERT,
-    bir_envty_includes_vs_EMPTY, PULL_EXISTS, PULL_FORALL, bir_type_is_Imm_def] >>
+    bir_envty_includes_vs_EMPTY, bir_ext_envty_includes_exts_UNION, bir_ext_envty_includes_exts_INSERT,
+    bir_ext_envty_includes_exts_EMPTY, PULL_EXISTS, PULL_FORALL, bir_type_is_Imm_def] >>
   REPEAT STRIP_TAC >>
   FULL_SIMP_TAC (std_ss++bir_val_ss) [type_of_bir_val_EQ_ELIMS, bir_type_is_Imm_def]
 ) >- (
@@ -742,8 +750,7 @@ NTAC 4 GEN_TAC >> Induct >> (
   ASM_SIMP_TAC (std_ss++bir_val_ss) [bir_eval_ifthenelse_REWRS] >>
   METIS_TAC[]
 ) >- (
-  fs[bir_eval_extget_def] >>
-  metis_tac[]
+  METIS_TAC[bir_ext_in_ext_envty_ext_env_IMP]
 ) >- (
   ASM_SIMP_TAC (std_ss++bir_val_ss) [bir_eval_load_BASIC_REWR] >>
   rename1 `bir_load_from_mem vt ity at mmap en (b2n i)` >>
@@ -769,10 +776,9 @@ NTAC 4 GEN_TAC >> Induct >> (
   ASM_SIMP_TAC (std_ss++bir_val_ss) []
 ));
 
-(* TODO: move elsewhere *)
-open bir_env_oldTheory;
+(* TODO: needs bir_env_oldTheory *)
 val type_of_bir_exp_THM_with_init_vars = store_thm ("type_of_bir_exp_THM_with_init_vars",
-  ``!ext_map env e ty ext_st. (type_of_bir_exp ext_map e = SOME ty) ==>
+  ``!ext_map env e ty ext_st. (type_of_bir_exp e = SOME ty) ==>
                (bir_env_vars_are_initialised env (bir_vars_of_exp e)) ==>
                (?va. (bir_eval_exp ext_map e env ext_st = SOME va) /\ (type_of_bir_val va = ty))``,
   METIS_TAC [type_of_bir_exp_THM_with_envty, bir_env_vars_are_initialised_EQ_envty, bir_env_satisfies_envty_of_env]
@@ -891,8 +897,8 @@ Induct_on `e` >> (
    More subtly, one needs also make sure that variables occuring in the expression
    are having consistent type annotations. This is expressed as follows: *)
 
-val bir_exp_is_well_typed_def = Define `bir_exp_is_well_typed ext_map e <=>
-  (IS_SOME (type_of_bir_exp ext_map e) /\
+val bir_exp_is_well_typed_def = Define `bir_exp_is_well_typed e <=>
+  (IS_SOME (type_of_bir_exp e) /\
    bir_vs_consistent (bir_vars_of_exp e))`
 
 
